RedisProof/Finished/ProofLayer1/Layer1/dictGenHashFunction/LowSpec.v
@@ -1,0 +1,49 @@
+Require Import Bottom.Spec.
+Require Import CommonDeps.
+Require Import DataTypes.
+Require Import GlobalDefs.
+
+Local Open Scope string_scope.
+Local Open Scope Z_scope.
+
+Section Layer1_dictGenHashFunction_LowSpec.
+
+  Context `{int_ptr: IntPtrCast}.
+
+  (* Fixpoint dictGenHashFunction_loop_0_low (buf_addr_0: Ptr) (len_addr_0: Z) (hash_0: Z) (arg_dummy0: Z) (arg_dummy1: Z) (st: RData) : (option (Ptr * Z * Z * Z * Z * RData)) :=
+    if (len_addr_0 <>? (0))
+    then (
+      when v_0, st_0 == ((load_RData 1 buf_addr_0 st));
+      (dictGenHashFunction_loop_0_low (ptr_offset buf_addr_0 1) (len_addr_0 + ((-1))) (((hash_0 << (5)) + (hash_0)) + (v_0)) arg_dummy0 arg_dummy1 st_0))
+    else (Some (buf_addr_0, len_addr_0, hash_0, hash_0, 0, st)). *)
+
+  Program Fixpoint dictGenHashFunction_loop_0_low
+        (buf_addr_0 : Ptr)
+        (len_addr_0 hash_0 arg_dummy0 arg_dummy1 : Z)
+        (st : RData)
+  {measure (Z.to_nat (len_addr_0))}
+  : (option (Ptr * Z * Z * Z * Z * RData)) :=
+    relyp (len_addr_0 >= 0);
+      match len_addr_0 =d 0 with
+      | left _   => Some (buf_addr_0, len_addr_0, hash_0, hash_0, 0, st)
+      | right Hlt =>
+        (when v_0, st_0 == ((load_RData 1 buf_addr_0 st));
+        (dictGenHashFunction_loop_0_low (ptr_offset buf_addr_0 1) (len_addr_0 + ((-1))) (((hash_0 << (5)) + (hash_0)) + (v_0)) arg_dummy0 arg_dummy1 st_0))
+      end.
+  Next Obligation.
+    (* Goal: Z.to_nat (size - i_0 * 2) < Z.to_nat (size - i_0)
+      Context: ~ i_0 <= 0       => i_0 > 0
+               ~ i_0 >= size    => i_0 < size  *)
+    lia.
+  Defined.
+
+  Definition dictGenHashFunction_spec_low (buf: Ptr) (len: Z) (st: RData) : (option (Z * RData)) :=
+    match ((dictGenHashFunction_loop_0_low buf len 5381 0 0 st)) with
+    | (Some (buf_addr_0_after, len_addr_0_after, hash_0_after, hash_0, v_1, st_0)) => (Some (hash_0, st_0))
+    | None => None
+    end.
+
+End Layer1_dictGenHashFunction_LowSpec.
+
+#[global] Hint Unfold dictGenHashFunction_loop_0_low: spec.
+#[global] Hint Unfold dictGenHashFunction_spec_low: spec.
